Experiments/Test_Suite.thy
@@ -666,4 +666,110 @@ proof -
 qed
 
 
+
+
+
+
+
+
+
+lemma passes_test_suite_exhaustiveness :
+  assumes "observable M"
+  and     "completely_specified M"
+  and     "is_sufficient_for_reduction_testing (Test_Suite prs tps rd_targets atcs) M m"
+  and     "passes_test_suite M (Test_Suite prs tps rd_targets atcs) M'"
+  and     "observable M'"
+  and     "inputs M' = inputs M"
+shows     "L M' \<subseteq> L M"
+proof (rule ccontr)
+  assume "\<not> L M' \<subseteq> L M"
+
+
+  have t1: "(initial M, initial_preamble M) \<in> prs" 
+    using assms(3) unfolding is_sufficient_for_reduction_testing.simps by blast
+  have t2: "\<And> q P. (q, P) \<in> prs \<Longrightarrow> is_preamble P M q \<and> tps q \<noteq> {}"
+    using assms(3) unfolding is_sufficient_for_reduction_testing.simps by force
+  have t3: "\<And> q1 q2 A d1 d2. (A, d1, d2) \<in> atcs (q1, q2) \<Longrightarrow> (A, d2, d1) \<in> atcs (q2, q1) \<and> is_separator M q1 q2 A d1 d2"
+    using assms(3) unfolding is_sufficient_for_reduction_testing.simps by force 
+  have t4: "\<And> q1 q2 . q1 \<in> fst ` prs \<Longrightarrow> q2 \<in> fst ` prs \<Longrightarrow> q1 \<noteq> q2 \<Longrightarrow> atcs (q1, q2) \<noteq> {} \<Longrightarrow> [] \<in> tps q1 \<and> [] \<in> tps q2 \<and> q1 \<in> rd_targets (q2, []) \<and> q2 \<in> rd_targets (q1, [])"
+    using assms(3) unfolding is_sufficient_for_reduction_testing.simps by auto 
+  
+
+
+
+  obtain RepSets where
+       t5: "\<And>q. q \<in> FSM.nodes M \<Longrightarrow> (\<exists>d\<in>set RepSets. q \<in> fst d)"
+   and "\<And> d. d \<in> set RepSets \<Longrightarrow> fst d \<subseteq> FSM.nodes M \<and> snd d \<subseteq> fst d \<and> (\<forall>q1 q2. q1 \<in> fst d \<longrightarrow> q2 \<in> fst d \<longrightarrow> q1 \<noteq> q2 \<longrightarrow> atcs (q1, q2) \<noteq> {})"
+   and t6: "\<And> q. q \<in> fst ` prs \<Longrightarrow> tps q \<subseteq> {p1 . \<exists> p2 d . (p1@p2,d) \<in> m_traversal_paths_with_witness M q RepSets m} \<and> fst ` (m_traversal_paths_with_witness M q RepSets m) \<subseteq> tps q"
+   and rs_paths': "\<And> q p d.
+          q \<in> fst ` prs \<Longrightarrow>
+          (p, d) \<in> m_traversal_paths_with_witness M q RepSets m \<Longrightarrow>
+          (\<forall>p1 p2 p3.
+              p = p1 @ p2 @ p3 \<longrightarrow>
+              p2 \<noteq> [] \<longrightarrow>
+              target q p1 \<in> fst d \<longrightarrow>
+              target q (p1 @ p2) \<in> fst d \<longrightarrow>
+              target q p1 \<noteq> target q (p1 @ p2) \<longrightarrow>
+              p1 \<in> tps q \<and> p1 @ p2 \<in> tps q \<and> target q p1 \<in> rd_targets (q, p1 @ p2) \<and> target q (p1 @ p2) \<in> rd_targets (q, p1)) \<and>
+          (\<forall>p1 p2 q'.
+              p = p1 @ p2 \<longrightarrow>
+              q' \<in> fst ` prs \<longrightarrow>
+              target q p1 \<in> fst d \<longrightarrow>
+              q' \<in> fst d \<longrightarrow> target q p1 \<noteq> q' \<longrightarrow> p1 \<in> tps q \<and> [] \<in> tps q' \<and> target q p1 \<in> rd_targets (q', []) \<and> q' \<in> rd_targets (q, p1))"
+    using assms(3) unfolding is_sufficient_for_reduction_testing.simps by force
+
+  have t7: "\<And> d. d \<in> set RepSets \<Longrightarrow> fst d \<subseteq> FSM.nodes M"
+  and  t8: "\<And> d. d \<in> set RepSets \<Longrightarrow> snd d \<subseteq> fst d"
+  and  t9: "\<And> d q1 q2. d \<in> set RepSets \<Longrightarrow> q1 \<in> fst d \<Longrightarrow> q2 \<in> fst d \<Longrightarrow> q1 \<noteq> q2 \<Longrightarrow> atcs (q1, q2) \<noteq> {}"
+    using \<open>\<And> d. d \<in> set RepSets \<Longrightarrow> fst d \<subseteq> FSM.nodes M \<and> snd d \<subseteq> fst d \<and> (\<forall>q1 q2. q1 \<in> fst d \<longrightarrow> q2 \<in> fst d \<longrightarrow> q1 \<noteq> q2 \<longrightarrow> atcs (q1, q2) \<noteq> {})\<close>
+    by blast+
+
+  have t10: "\<And> q p d p1 p2 p3.
+              q \<in> fst ` prs \<Longrightarrow>
+              (p, d) \<in> m_traversal_paths_with_witness M q RepSets m \<Longrightarrow>
+              p = p1 @ p2 @ p3 \<Longrightarrow>
+              p2 \<noteq> [] \<Longrightarrow>
+              target q p1 \<in> fst d \<Longrightarrow>
+              target q (p1 @ p2) \<in> fst d \<Longrightarrow>
+              target q p1 \<noteq> target q (p1 @ p2) \<Longrightarrow>
+              p1 \<in> tps q \<and> p1 @ p2 \<in> tps q \<and> target q p1 \<in> rd_targets (q, p1 @ p2) \<and> target q (p1 @ p2) \<in> rd_targets (q, p1)"
+    using rs_paths' by blast
+
+  have t11: "\<And> q p d p1 p2 q'.
+              q \<in> fst ` prs \<Longrightarrow>
+              (p, d) \<in> m_traversal_paths_with_witness M q RepSets m \<Longrightarrow>
+              p = p1 @ p2 \<Longrightarrow>
+              q' \<in> fst ` prs \<Longrightarrow>
+              target q p1 \<in> fst d \<Longrightarrow>
+              q' \<in> fst d \<Longrightarrow> 
+              target q p1 \<noteq> q' \<Longrightarrow> 
+              p1 \<in> tps q \<and> [] \<in> tps q' \<and> target q p1 \<in> rd_targets (q', []) \<and> q' \<in> rd_targets (q, p1)"
+    using rs_paths' by blast
+  
+
+
+
+  obtain io where "minimal_sequence_to_failure_extending_preamble M M' prs io"
+    using minimal_sequence_to_failure_extending_preamble_ex[OF t1 \<open>\<not> L M' \<subseteq> L M\<close>] by blast
+
+  then have "sequence_to_failure_extending_preamble M M' prs io" 
+            "\<And> io'. sequence_to_failure_extending_preamble M M' prs io' \<Longrightarrow> length io \<le> length io'"
+    unfolding minimal_sequence_to_failure_extending_preamble_def
+    by blast+
+
+  obtain q P p where "q \<in> nodes M"
+                 and "(q,P) \<in> prs"
+                 and "path P (initial P) p"
+                 and "target (initial P) p = q"
+                 and "((p_io p) @ butlast io) \<in> L M  " 
+                 and "((p_io p) @ io) \<notin> L M"
+                 and "((p_io p) @ io) \<in> L M'"
+    using \<open>sequence_to_failure_extending_preamble M M' prs io\<close>
+    unfolding sequence_to_failure_extending_preamble_def 
+    by blast
+
+              
+
+
+
 end
